[RelationalIO] Separate public and private inputs
Fix the precondition to say that public inputs must be equal, not all
inputs.

theories/Relational/RelationalIO.v
@@ -113,39 +113,53 @@ End IOs.
 
 Section NI_IO.
   Section IOHigh.
-    Context {Inp Oup : Type}.
+    Context {IPub IPriv Oup : Type}.
 
     Inductive IOS : Type := ReadLow : IOS | ReadHigh : IOS | Write : Oup -> IOS.
     Definition IOAr (op : IOS) : Type :=
       match op with
-      | ReadLow => Inp
-      | ReadHigh => Inp
+      | ReadLow => IPub
+      | ReadHigh => IPriv
       | Write _ => unit
       end.
 
     Definition IO := @Free IOS IOAr.
 
-    Definition readLow : IO Inp := op _ ReadLow.
-    Definition readHigh : IO Inp := op _ ReadHigh.
+    Definition readLow : IO IPub := op _ ReadLow.
+    Definition readHigh : IO IPriv := op _ ReadHigh.
     Definition write (o:Oup) : IO unit := op _ (Write o).
-  End IOHigh.
-  Context {I1 O1 I2 O2 : Type}.
 
-  Program Definition wop1' (s:IOS) : @Wun I1 I2 O1 O2 (IOAr s) :=
+    Inductive IOTriple : Type := InpPub : IPub -> IOTriple
+                               | InpPriv : IPriv -> IOTriple
+                               | Out : Oup -> IOTriple.
+  End IOHigh.
+
+  Context {IPub1 IPriv1 O1 IPub2 IPriv2 O2 : Type}.
+  Notation "i1 ⊕ i2 ⊕ o" := (@IOTriple i1 i2 o) (at level 65, i2 at next level).
+
+  Let Es1 := list (IPub1 ⊕ IPriv1 ⊕ O1).
+  Let Es2 := list (IPub2 ⊕ IPriv2 ⊕ O2).
+  Let Es12 := Es1 × Es2.
+  Let carrier := Es12 -> SProp.
+
+  Definition Wun' :=
+    @MonoCont carrier (@Pred_op_order _) (@Pred_op_order_prorder _).
+
+  Program Definition wop1' (s:IOS) : Wun' (IOAr s) :=
     match s with
-    | ReadLow => ⦑fun p h => forall i, p i ⟨ inl i :: nfst h, nsnd h ⟩⦒
-    | ReadHigh => ⦑fun p h => forall i, p i ⟨ inl i :: nfst h, nsnd h ⟩⦒
-    | Write o => ⦑fun p h => p tt ⟨ inr o :: nfst h, nsnd h ⟩⦒
+    | ReadLow => ⦑fun p h => forall i, p i ⟨ InpPub i :: nfst h, nsnd h ⟩⦒
+    | ReadHigh => ⦑fun p h => forall i, p i ⟨ InpPriv i :: nfst h, nsnd h ⟩⦒
+    | Write o => ⦑fun p h => p tt ⟨ Out o :: nfst h, nsnd h ⟩⦒
     end.
   Next Obligation. move=> ? ? H ? H0 ?; apply H ; apply H0. Qed.
   Next Obligation. move=> ? ? H ? H0 ?; apply H ; apply H0. Qed.
   Next Obligation. move=> ? ? H ? H0 ; apply H; apply H0. Qed.
 
-  Program Definition wop2' (s:IOS) : @Wun I1 I2 O1 O2 (IOAr s) :=
+  Program Definition wop2' (s:IOS) : Wun' (IOAr s) :=
     match s with
-    | ReadLow => ⦑fun p h => forall i, p i ⟨ nfst h, inl i :: nsnd h ⟩⦒
-    | ReadHigh => ⦑fun p h => forall i, p i ⟨ nfst h, inl i :: nsnd h ⟩⦒
-    | Write o => ⦑fun p h => p tt ⟨ nfst h, inr o :: nsnd h ⟩⦒
+    | ReadLow => ⦑fun p h => forall i, p i ⟨ nfst h, InpPub i :: nsnd h ⟩⦒
+    | ReadHigh => ⦑fun p h => forall i, p i ⟨ nfst h, InpPriv i :: nsnd h ⟩⦒
+    | Write o => ⦑fun p h => p tt ⟨ nfst h, Out o :: nsnd h ⟩⦒
     end.
   Next Obligation. move=> ? ? H ? H0 ?; apply H ; apply H0. Qed.
   Next Obligation. move=> ? ? H ? H0 ?; apply H ; apply H0. Qed.
@@ -158,29 +172,55 @@ Section NI_IO.
     all: apply SPropAxioms.sprop_ext; do 2 split => //.
   Qed.
 
-  Let M1 := @IO I1 O1.
-  Let M2 := @IO I2 O2.
-  Let Wrel := Wrel (@Wun I1 I2 O1 O2).
+  Let M1 := @IO IPub1 IPriv1 O1.
+  Let M2 := @IO IPub2 IPriv2 O2.
+  Let Wrel := Wrel Wun'.
 
   Definition θIO' :=
-    commute_effObs Wun M1 M2 _ _
-                   (fromFreeCommute Wun wop1' wop2' io1_io2_commutation').
+    commute_effObs Wun' M1 M2 _ _
+                   (fromFreeCommute Wun' wop1' wop2' io1_io2_commutation').
+
+  Program Definition fromPrePost' {A1 A2}
+          (pre : Es1 -> Es2 -> SProp)
+          (post : A1 -> Es1 -> Es1 -> A2 -> Es2 -> Es2 -> SProp)
+    : dfst (Wrel ⟨A1,A2⟩) :=
+    ⦑fun p h => pre (nfst h) (nsnd h) s/\
+                 forall a1 a2 h', post a1 (nfst h) (nfst h') a2 (nsnd h) (nsnd h')
+                            -> p ⟨a1, a2⟩ h'⦒.
+  Next Obligation. split; case: H0 => // ? Hy *; apply H, Hy=> //. Qed.
 End NI_IO.
 
 Section NI_Examples.
   (* For the purpose of examples, let's just have one type of inputs and outputs *)
   Context (Ty : Type).
-  Let θIO' := @θIO' Ty Ty Ty Ty.
-  Let readHigh := @readHigh Ty Ty.
-  Let readLow := @readLow Ty Ty.
-  Let write := @write Ty Ty.
+  Let θIO' := @θIO' Ty Ty Ty Ty Ty Ty.
+  Let Wun' := @Wun' Ty Ty Ty Ty Ty Ty.
+  Let readHigh := @readHigh Ty Ty Ty.
+  Let readLow := @readLow Ty Ty Ty.
+  Let write := @write Ty Ty Ty.
+  Let IOTriple := @IOTriple Ty Ty Ty.
 
   Notation "⊨ ⦃ pre ⦄ c1 ≈ c2 ⦃ post ⦄" :=
-    (semantic_judgement _ _ _ θIO' _ _ c1 c2 (fromPrePost pre post)).
+    (semantic_judgement _ _ _ θIO' _ _ c1 c2 (fromPrePost' pre post)).
+
+  Definition isPubInp (i : IOTriple) : bool := match i with
+                                           | InpPub _ => true
+                                           | _ => false
+                                           end.
+
+  Definition isPrivInp (i : IOTriple) : bool := match i with
+                                            | InpPriv _ => true
+                                            | _ => false
+                                            end.
+
+  Definition isOut (i : IOTriple) : bool := match i with
+                                        | Out _ => true
+                                        | _ => false
+                                        end.
 
   (* Noninterference property *)
   Definition NI {A : Type} (c : IO A) :=
-    ⊨ ⦃ fun h1 h2 => h1 ≡ h2 ⦄
+    ⊨ ⦃ fun h1 h2 => filter isPubInp h1 ≡ filter isPubInp h2 ⦄
       c ≈ c
       ⦃ fun a1 h1 h1' a2 h2 h2' => h1' ≡ h2' s/\ a1 ≡ a2 ⦄.
 
